rt aspec+ainvs: AInvs for AARCH64
Modify the assumptions of the DetSchedSchedule_AI_handle_hypervisor_fault
locale in order to accommodate the AARCH64 versions of handle_hypervisor_fault
and handle_reserved_irq, which call handle_fault, in contrast with the ARM and
RISCV64 versions of these functions, which are noops. Remove several
unnecessary assumptions from the DetSchedSchedule_AI locale.

Introduce locales in the AInvs theory file in order to accommodate the AARCH64
versions of handle_hypervisor_fault and handle_reserved_irq. Add the
architecture-dependent theory file ArchAInvs to interpret the locales added to
AInvs, importing the ArchAInvs theory file wherever AInvs.AInvs was previously
imported.

Add an assert to guarded_switch_to in ASpec stating that the thread that we
switch to is in the current domain, in order to simplify the invariant proofs
in ArchFPU_AI and ArchVCPU_AI, noting that the corres rule for
guarded_switch_to already has an abstract guard from which the truth of the
assert follows straightforwardly.

Signed-off-by: Michael McInerney <michael.mcinerney@proofcraft.systems>

spec/abstract/Schedule_A.thy
@@ -36,6 +36,11 @@ definition guarded_switch_to :: "obj_ref \<Rightarrow> (unit, 'z::state_ext) s_m
      scp \<leftarrow> assert_opt sc_opt;
      sched \<leftarrow> gets (schedulable thread);
      assert sched;
+     \<comment> \<open>to simplify the proofs of the invariants related to VCPUs and FPUs, we assert that the
+         thread that we switch to is in the current domain.\<close>
+     d \<leftarrow> gets cur_domain;
+     next_domain \<leftarrow> thread_get tcb_domain thread;
+     assert (next_domain = d);
      switch_to_thread thread
    od"
 
