proof/invariant-abstract/AARCH64/ArchAInvs.thy
@@ -1,0 +1,68 @@
+(*
+ * Copyright 2026, Proofcraft Pty Ltd
+ *
+ * SPDX-License-Identifier: GPL-2.0-only
+ *)
+
+theory ArchAInvs
+imports AInvs
+begin
+
+context Arch begin arch_global_naming
+
+crunch handle_hypervisor_fault, handle_reserved_irq
+  for schact_is_not_rct[wp]: "\<lambda>s. \<not> schact_is_rct s"
+  (wp: crunch_wps)
+
+crunch do_machine_op
+  for schact_is_rct_ct_in_state_activatable[wp]: "\<lambda>s. schact_is_rct s \<longrightarrow> ct_in_state activatable s"
+  (wp: hoare_vcg_imp_lift')
+
+lemma handle_hypervisor_fault_schact_is_rct_ct_in_state_activatable[wp]:
+  "handle_hypervisor_fault t fault \<lbrace>\<lambda>s. schact_is_rct s \<longrightarrow> ct_in_state activatable s\<rbrace>"
+  supply if_split[split del]
+  by (cases fault; wpsimp)
+
+lemma set_vcpu_schact_is_rct_ct_in_state_activatable[wp]:
+  "set_vcpu ptr vcpu \<lbrace>\<lambda>s. schact_is_rct s \<longrightarrow> ct_in_state activatable s\<rbrace>"
+  unfolding set_vcpu_def
+  apply (wpsimp wp: set_object_wp_strong)
+  apply (clarsimp simp: ct_in_state_def st_tcb_at_def obj_at_def)
+  done
+
+crunch vgic_update_lr
+  for schact_is_rct_ct_in_state_activatable[wp]: "\<lambda>s. schact_is_rct s \<longrightarrow> ct_in_state activatable s"
+  (simp: ct_in_state_def)
+
+lemma vgic_maintenance_schact_is_rct_ct_in_state_activatable[wp]:
+  "vgic_maintenance \<lbrace>\<lambda>s. schact_is_rct s \<longrightarrow> ct_in_state activatable s\<rbrace>"
+  unfolding vgic_maintenance_def
+  supply if_split[split del]
+  apply (wpsimp wp: thread_get_wp' | wp (once) hoare_drop_imps)+
+  apply (clarsimp simp: ct_in_state_def st_tcb_at_def obj_at_def split: if_splits)
+  done
+
+crunch handle_hypervisor_fault, handle_reserved_irq
+  for schact_is_rct_ct_in_state_activatable[wp]: "\<lambda>s. schact_is_rct s \<longrightarrow> ct_in_state activatable s"
+  and cur_sc[wp]: "\<lambda>s. P (cur_sc s)"
+  and is_active_sc[wp]: "\<lambda>s. P (is_active_sc sc_ptr s)"
+
+crunch handle_hypervisor_fault, handle_reserved_irq
+  for ct_not_in_release_q[wp]: ct_not_in_release_q
+  (wp: crunch_wps)
+
+end
+
+global_interpretation AInvs_AI?: AInvs_AI
+proof goal_cases
+  interpret Arch .
+  case 1 show ?case by (unfold_locales; (solves wpsimp)?)
+qed
+
+global_interpretation AInvs_AI_det_ext?: AInvs_AI_det_ext
+proof goal_cases
+  interpret Arch .
+  case 1 show ?case by (unfold_locales; wpsimp)
+qed
+
+end
