proof/invariant-abstract/AARCH64/ArchInterruptAcc_AI.thy
@@ -19,12 +19,17 @@ named_theorems InterruptAcc_AI_assms
 lemma dmo_maskInterrupt_invs [InterruptAcc_AI_assms]:
   "\<lbrace>all_invs_but_valid_irq_states_for irq and (\<lambda>s. state = interrupt_states s irq)\<rbrace>
    do_machine_op (maskInterrupt (state = IRQInactive) irq)
-   \<lbrace>\<lambda>rv. invs\<rbrace>"
-  apply (simp add: do_machine_op_def split_def maskInterrupt_def)
-  apply wp
-  apply (clarsimp simp: in_monad invs_def valid_state_def all_invs_but_valid_irq_states_for_def
-                        valid_irq_states_but_def valid_irq_masks_but_def valid_machine_state_def
-                        cur_tcb_def valid_irq_states_def valid_irq_masks_def)
+   \<lbrace>\<lambda>_. invs\<rbrace>"
+  by (wpsimp simp: do_machine_op_def maskInterrupt_def in_monad invs_def valid_state_def
+                   all_invs_but_valid_irq_states_for_def valid_irq_states_but_def
+                   valid_irq_masks_but_def valid_machine_state_def cur_tcb_def cur_sc_tcb_def
+                   valid_irq_states_def valid_irq_masks_def)
+
+lemma getCurrentTime_invs[wp]:
+  "do_machine_op getCurrentTime \<lbrace>invs\<rbrace>"
+  unfolding getCurrentTime_def
+  apply (wpsimp wp: dmo_invs)
+  apply (simp add: in_monad)
   done
 
 crunch handle_spurious_irq
