proof/invariant-abstract/AARCH64/ArchRetype_AI.thy
@@ -157,7 +157,7 @@ lemma init_arch_objects_invs_from_restricted:
 
 
 lemma obj_bits_api_neq_0 [Retype_AI_assms]:
-  "ty \<noteq> Untyped \<Longrightarrow> 0 < obj_bits_api ty us"
+  "\<lbrakk>ty \<noteq> Untyped; ty \<noteq> SchedContextObject\<rbrakk> \<Longrightarrow> 0 < obj_bits_api ty us"
   unfolding obj_bits_api_def
   by (clarsimp simp: slot_bits_def default_arch_object_def bit_simps
                split: apiobject_type.splits aobject_type.splits)
@@ -178,6 +178,7 @@ lemma valid_untyped_helper [Retype_AI_assms]:
   assumes valid_c : "s  \<turnstile> c"
   and   cte_at  : "cte_wp_at ((=) c) q s"
   and     tyunt: "ty \<noteq> Structures_A.apiobject_type.Untyped"
+  and      tysc: "ty = SchedContextObject \<Longrightarrow> min_sched_context_bits \<le> us \<and> us \<le> untyped_max_bits"
   and   cover  : "range_cover ptr sz (obj_bits_api ty us) n"
   and   range  : "is_untyped_cap c \<Longrightarrow> usable_untyped_range c \<inter> {ptr..ptr + of_nat (n * 2 ^ (obj_bits_api ty us)) - 1} = {}"
   and     pn   : "pspace_no_overlap_range_cover ptr sz s"
@@ -192,9 +193,10 @@ proof -
        (erule pspace_no_overlapC [OF pn _ _ cover vp])
   note [simp del] = atLeastAtMost_iff atLeastatMost_subset_iff atLeastLessThan_iff
                     Int_atLeastAtMost atLeastatMost_empty_iff
+  note [simp del] = atLeastAtMost_simps
   have cover':"range_cover ptr sz (obj_bits (default_object ty dev us (cur_domain s))) n"
-    using cover tyunt
-    by (clarsimp simp:obj_bits_dev_irr)
+    using cover tyunt tysc
+    by (clarsimp simp: obj_bits_dev_irr)
 
   show ?thesis
     using cover valid_c range usable_range_emptyD[where cap = c] cte_at
@@ -207,16 +209,15 @@ proof -
     apply (clarsimp simp:valid_untyped_def is_cap_simps obj_at_def split:if_split_asm)
      apply (thin_tac "\<forall>x. Q x" for Q)
      apply (frule retype_addrs_obj_range_subset_strong[where dev=dev, OF _ _ tyunt])
-      apply (simp add: obj_bits_dev_irr tyunt)
+       apply (simp add: obj_bits_dev_irr tyunt)
+      apply (clarsimp simp: tysc)
      apply (frule usable_range_subseteq)
       apply (simp add:is_cap_simps)
      apply (clarsimp simp:cap_aligned_def split:if_split_asm)
      apply (frule aligned_ranges_subset_or_disjoint)
       apply (erule retype_addrs_aligned[where sz = sz])
-        apply (simp add: range_cover_def)
-       apply (simp add: range_cover_def word_bits_def)
-      apply (simp add: range_cover_def)
-     apply (clarsimp simp: default_obj_range Int_ac tyunt
+        apply (simp add: range_cover_def word_bits_def)+
+     apply (clarsimp simp: default_obj_range Int_ac tyunt tysc
                     split: if_split_asm)
      apply (elim disjE)
       apply (drule(2) subset_trans[THEN disjoint_subset2])
@@ -232,9 +233,10 @@ proof -
     apply (rule context_conjI)
      apply clarsimp
      apply (frule retype_addrs_obj_range_subset[OF _ cover' tyunt])
+      apply (simp add: tysc)
      apply (frule aligned_ranges_subset_or_disjoint)
       apply (erule retype_addrs_aligned[where sz = sz]; simp add: range_cover_def word_bits_def)
-     apply (clarsimp simp: default_obj_range Int_ac tyunt)
+     apply (clarsimp simp: default_obj_range Int_ac tyunt tysc)
      apply (erule disjE)
       apply (simp add: cte_wp_at_caps_of_state)
       apply (drule cn[unfolded caps_no_overlap_def,THEN bspec,OF ranI])
@@ -276,10 +278,9 @@ lemma valid_cap:
     "(s::'state_ext state) \<turnstile> cap \<and> untyped_range cap \<inter> {ptr .. (ptr && ~~ mask sz) + 2 ^ sz - 1} = {}"
   shows "s' \<turnstile> cap"
   proof -
-  note blah[simp del] = atLeastAtMost_iff atLeastatMost_subset_iff atLeastLessThan_iff
-        Int_atLeastAtMost atLeastatMost_empty_iff
+  note [simp del] = atLeastAtMost_simps
   have cover':"range_cover ptr sz (obj_bits (default_object ty dev us (cur_domain s))) n"
-    using cover tyunt
+    using cover tyunt tysc
     by (clarsimp simp: obj_bits_dev_irr)
   show ?thesis
     unfolding valid_cap_def
@@ -290,11 +291,11 @@ lemma valid_cap:
     apply (clarsimp simp add: valid_untyped_def ps_def s'_def)
     apply (rule conjI)
      apply clarsimp
-     apply (drule disjoint_subset [OF retype_addrs_obj_range_subset [OF _ cover' tyunt]])
+     apply (drule (1) disjoint_subset [OF retype_addrs_obj_range_subset [OF _ cover' tyunt tysc[THEN conjunct1, THEN impI]]])
       apply (simp add: Int_ac p_assoc_help[symmetric])
      apply fastforce
     apply clarsimp
-    apply (drule disjoint_subset [OF retype_addrs_obj_range_subset [OF _ cover' tyunt]])
+     apply (drule (1) disjoint_subset [OF retype_addrs_obj_range_subset [OF _ cover' tyunt tysc[THEN conjunct1, THEN impI]]])
      apply (simp add: Int_ac p_assoc_help[symmetric])
     apply fastforce
     done
@@ -699,7 +700,7 @@ lemma valid_table_caps:
 
 lemma caps_of_state':
   "caps_of_state s p = Some cap \<Longrightarrow> caps_of_state s' p = Some cap"
-  by (fastforce simp: F cte_wp_at_cases s'_def ps_def orthr)
+  by (fastforce simp: cte_wp_at_cases s'_def ps_def orthr caps_of_state_Some_simp)
 
 lemma valid_vs_lookup:
   "valid_vs_lookup s \<Longrightarrow> valid_vs_lookup s'"
@@ -753,8 +754,8 @@ lemma pspace_in_kernel_window:
   apply (simp add: pspace_in_kernel_window_def s'_def ps_def)
   apply (clarsimp simp: region_in_kernel_window_def
                    del: ballI)
-  apply (drule retype_addrs_mem_subset_ptr_bits[OF cover tyunt])
-  apply (fastforce simp: field_simps obj_bits_dev_irr tyunt)
+  apply (drule retype_addrs_mem_subset_ptr_bits[OF cover tyunt tysc[THEN conjunct1, simplified atomize_imp]])
+  apply (fastforce simp: field_simps obj_bits_dev_irr tyunt tysc)
   done
 
 lemma pspace_respects_device_region:
@@ -762,16 +763,17 @@ lemma pspace_respects_device_region:
       and cap_refs_resp_dev: "cap_refs_respects_device_region s"
   shows "pspace_respects_device_region s'"
   proof -
-    note blah[simp del] = untyped_range.simps usable_untyped_range.simps atLeastAtMost_iff
-          atLeastatMost_subset_iff atLeastLessThan_iff
-          Int_atLeastAtMost atLeastatMost_empty_iff split_paired_Ex
+    note [simp del] = untyped_range.simps usable_untyped_range.simps atLeastAtMost_iff
+                      atLeastatMost_subset_iff atLeastLessThan_iff
+                      Int_atLeastAtMost atLeastatMost_empty_iff split_paired_Ex
   show ?thesis
   apply (cut_tac vp)
   apply (rule pspace_respects_device_regionI)
      apply (clarsimp simp add: pspace_respects_device_region_def s'_def ps_def
                         split: if_split_asm )
-      apply (drule retype_addrs_obj_range_subset[OF _ _ tyunt, where d'="cur_domain s"])
-       using cover tyunt
+      apply (drule retype_addrs_obj_range_subset[OF _ _ tyunt tysc[THEN conjunct1, simplified atomize_imp],
+                                                 where d'="cur_domain s"])
+       using cover tyunt tysc
        apply (simp add: obj_bits_api_def3 split: if_splits)
       apply (frule default_obj_dev[OF tyunt],simp)
       apply (drule(1) subsetD)
@@ -784,8 +786,9 @@ lemma pspace_respects_device_region:
      apply fastforce
     apply (clarsimp simp add: pspace_respects_device_region_def s'_def ps_def
                        split: if_split_asm )
-     apply (drule retype_addrs_obj_range_subset[OF _ _ tyunt, where d'="cur_domain s"])
-      using cover tyunt
+     apply (drule retype_addrs_obj_range_subset[OF _ _ tyunt tysc[THEN conjunct1, simplified atomize_imp],
+                                                where d'="cur_domain s"])
+      using cover tyunt tysc
       apply (simp add: obj_bits_api_def4 split: if_splits)
      apply (frule default_obj_dev[OF tyunt],simp)
       apply (drule(1) subsetD)
@@ -838,7 +841,6 @@ lemma post_retype_invs:
   using equal_kernel_mappings valid_global_vspace_mappings
   apply (clarsimp simp: invs_def post_retype_invs_def valid_state_def
                      unsafe_rep2 null_filter valid_idle
-                     valid_reply_caps valid_reply_masters
                      valid_global_refs valid_arch_state valid_cur_fpu'
                      valid_irq_node_def obj_at_pres
                      valid_arch_caps valid_global_objs_def
@@ -847,7 +849,7 @@ lemma post_retype_invs:
                      valid_mdb_rep2 mdb_and_revokable
                      valid_pspace cur_tcb only_idle
                      valid_kernel_mappings valid_asid_map
-                     valid_ioc vms
+                     valid_ioc vms cur_sc_tcb
                      pspace_in_kernel_window
                      pspace_respects_device_region
                      cap_refs_respects_device_region
@@ -910,6 +912,7 @@ lemma retype_region_plain_invs:
       and region_in_kernel_window {ptr .. (ptr &&~~ mask sz) + 2 ^ sz - 1}
       and (\<lambda>s. \<exists>slot. cte_wp_at (\<lambda>c.  {ptr..(ptr && ~~ mask sz) + (2 ^ sz - 1)} \<subseteq> cap_range c \<and> cap_is_device c = dev) slot s)
       and K (ty = Structures_A.CapTableObject \<longrightarrow> 0 < us)
+      and K (ty = SchedContextObject \<longrightarrow>  min_sched_context_bits \<le> us \<and> us \<le> untyped_max_bits)
       and K (range_cover ptr sz (obj_bits_api ty us) n)\<rbrace>
       retype_region ptr n us ty dev \<lbrace>\<lambda>rv. invs\<rbrace>"
   apply (rule hoare_strengthen_post[OF retype_region_post_retype_invs])
@@ -937,8 +940,8 @@ lemma invs_irq_state_independent:
    = invs s"
   by (clarsimp simp: irq_state_independent_A_def invs_def
                      valid_state_def valid_pspace_def valid_mdb_def valid_ioc_def valid_idle_def
-                     only_idle_def if_unsafe_then_cap_def valid_reply_caps_def
-                     valid_reply_masters_def valid_global_refs_def valid_arch_state_def
+                     only_idle_def if_unsafe_then_cap_def
+                     valid_global_refs_def valid_arch_state_def
                      valid_irq_node_def valid_irq_handlers_def valid_machine_state_def
                      valid_vspace_objs_def valid_arch_caps_def
                      valid_kernel_mappings_def equal_kernel_mappings_def
@@ -947,6 +950,40 @@ lemma invs_irq_state_independent:
                      cur_tcb_def sym_refs_def state_refs_of_def state_hyp_refs_of_def
                      swp_def valid_irq_states_def
               split: option.split)
+
+lemma invs_getCurrentTime_independent:
+  "invs (s\<lparr>machine_state := machine_state s\<lparr>time_state := f (time_state (machine_state s))\<rparr>\<rparr>)
+   = invs s"
+  "invs (s\<lparr>machine_state := machine_state s\<lparr>last_machine_time :=
+                            g (last_machine_time (machine_state s)) (time_state (machine_state s))\<rparr>\<rparr>)
+   = invs s"
+  by (clarsimp simp: getCurrentTime_independent_A_def invs_def
+                     valid_state_def valid_pspace_def valid_mdb_def valid_ioc_def valid_idle_def
+                     only_idle_def if_unsafe_then_cap_def valid_irq_states_def
+                     valid_global_refs_def valid_arch_state_def
+                     valid_irq_node_def valid_irq_handlers_def valid_machine_state_def
+                     valid_arch_caps_def valid_global_objs_def
+                     valid_kernel_mappings_def equal_kernel_mappings_def
+                     valid_asid_map_def vspace_at_asid_def
+                     pspace_in_kernel_window_def cap_refs_in_kernel_window_def
+                     cur_tcb_def cur_sc_tcb_def sym_refs_def state_refs_of_def
+                     swp_def valid_replies_pred_pspaceI; safe; clarsimp)+
+
+lemma invs_update_time_stamp_independent:
+  "invs (s\<lparr>cur_time := f (cur_time s)\<rparr>) = invs s"
+  "invs (s\<lparr>consumed_time := g (consumed_time s) (cur_time s)\<rparr>) = invs s"
+  "invs (s\<lparr>domain_time := h (domain_time)\<rparr>) = invs s"
+  by (clarsimp simp: update_time_stamp_independent_A_def invs_def
+                     valid_state_def valid_pspace_def valid_mdb_def valid_ioc_def valid_idle_def
+                     only_idle_def if_unsafe_then_cap_def valid_irq_states_def
+                     valid_global_refs_def valid_arch_state_def
+                     valid_irq_node_def valid_irq_handlers_def valid_machine_state_def
+                     valid_arch_caps_def valid_global_objs_def
+                     valid_kernel_mappings_def equal_kernel_mappings_def
+                     valid_asid_map_def vspace_at_asid_def ex_cte_cap_wp_to_def
+                     pspace_in_kernel_window_def cap_refs_in_kernel_window_def
+                     cur_tcb_def cur_sc_tcb_def sym_refs_def state_refs_of_def
+                     swp_def valid_replies_pred_pspaceI; safe; clarsimp)+
 
 crunch storeWord, clearMemory
   for irq_masks_inv[wp]: "\<lambda>s. P (irq_masks s)"
@@ -978,8 +1015,10 @@ lemma caps_region_kernel_window_imp:
   done
 
 crunch init_arch_objects
-  for irq_node[wp]: "\<lambda>s. P (interrupt_irq_node s)"
-  (wp: crunch_wps)
+  for pred_tcb_at[wp]: "\<lambda>s. N (pred_tcb_at proj P t s)"
+  and irq_node[wp]: "\<lambda>s. P (interrupt_irq_node s)"
+  and ct_in_state[wp]: "ct_in_state P"
+  (wp: crunch_wps ct_in_state_thread_state_lift)
 
 lemma init_arch_objects_excap:
   "\<lbrace>ex_cte_cap_wp_to P p\<rbrace>
@@ -987,15 +1026,22 @@ lemma init_arch_objects_excap:
    \<lbrace>\<lambda>rv s. ex_cte_cap_wp_to P p s\<rbrace>"
   by (wp ex_cte_cap_to_pres)
 
-crunch init_arch_objects
-  for pred_tcb_at[wp]: "pred_tcb_at proj P t"
-  (wp: crunch_wps)
-
 lemma valid_arch_mdb_detype:
   "valid_arch_mdb (is_original_cap s) (caps_of_state s) \<Longrightarrow>
             valid_arch_mdb (is_original_cap (detype (untyped_range cap) s))
          (\<lambda>p. if fst p \<in> untyped_range cap then None else caps_of_state s p)"
   by (auto simp: valid_arch_mdb_def)
+
+lemma hyp_live_default_object:
+  "ty \<noteq> Untyped \<Longrightarrow> \<not> hyp_live (default_object ty dev us dm)"
+  by (cases ty;
+      simp add: hyp_live_def default_object_def default_tcb_def default_arch_tcb_def
+                default_arch_object_def arch_live_def default_vcpu_def
+         split: aobject_type.splits)
+
+lemma arch_tcb_live_default_arch_tcb:
+  "\<not> arch_tcb_live default_arch_tcb"
+  by (simp add: arch_tcb_live_def default_arch_tcb_def)
 
 lemmas init_arch_objects_wps
     = init_arch_objects_cte_wp_at
@@ -1003,6 +1049,8 @@ lemmas init_arch_objects_wps
       init_arch_objects_cap_table
       init_arch_objects_excap
       init_arch_objects_pred_tcb_at
+      init_arch_objects_cur_thread
+      init_arch_objects_ct_in_state
 
 end
 
