proof/invariant-abstract/ARM/ArchAInvs.thy
@@ -1,0 +1,23 @@
+(*
+ * Copyright 2026, Proofcraft Pty Ltd
+ *
+ * SPDX-License-Identifier: GPL-2.0-only
+ *)
+
+theory ArchAInvs
+imports AInvs
+begin
+
+global_interpretation AInvs_AI?: AInvs_AI
+proof goal_cases
+  interpret Arch .
+  case 1 show ?case by (unfold_locales; (solves wpsimp)?)
+qed
+
+global_interpretation AInvs_AI_det_ext?: AInvs_AI_det_ext
+proof goal_cases
+  interpret Arch .
+  case 1 show ?case by (unfold_locales; wpsimp)
+qed
+
+end
