proof/invariant-abstract/Ipc_AI.thy
@@ -2894,17 +2894,14 @@ lemma ep_ntfn_cap_case_helper:
       R)"
   by (cases x, simp_all)
 
-crunch complete_signal, do_nbrecv_failed_transfer
+crunch do_nbrecv_failed_transfer
   for pred_tcb_at[wp]: "\<lambda>s. P (pred_tcb_at proj P' t s)"
   (wp: crunch_wps hoare_vcg_all_lift)
 
 lemma complete_signal_st_tcb_at[wp]:
   "complete_signal ntfnptr tptr \<lbrace>\<lambda>s. Q (st_tcb_at P t s)\<rbrace>"
   apply (clarsimp simp: complete_signal_def)
-  apply (rule bind_wp_fwd_skip, solves wpsimp)
-  apply (case_tac "ntfn_obj ntfn"; clarsimp)
-  apply (rule bind_wp_fwd_skip, solves wpsimp)+
-  apply wpsimp
+  apply (wpsimp wp: hoare_drop_imps hoare_vcg_all_lift)
   done
 
 lemmas thread_set_Pmdb = thread_set_cdt
