proof/invariant-abstract/RISCV64/ArchInterrupt_AI.thy
@@ -240,8 +240,10 @@ lemma (* handle_interrupt_invs *) [Interrupt_AI_assms]:
   apply (simp add: handle_interrupt_def)
   apply (rule conjI; rule impI)
    apply (simp add: do_machine_op_bind empty_fail_ackInterrupt_ARCH empty_fail_maskInterrupt_ARCH)
-   apply (wp dmo_maskInterrupt_invs maskInterrupt_invs_ARCH dmo_ackInterrupt send_signal_interrupt_states
-          | wpc | simp add: arch_mask_irq_signal_def)+
+   apply (wpsimp wp: dmo_maskInterrupt_invs maskInterrupt_invs_ARCH dmo_ackInterrupt
+                     send_signal_interrupt_states
+               simp: arch_mask_irq_signal_def when_def
+          split_del: if_split)+
        apply (wp get_cap_wp send_signal_interrupt_states)
       apply (rule_tac Q'="\<lambda>rv. invs and (\<lambda>s. st = interrupt_states s irq)" in hoare_post_imp)
        apply (clarsimp simp: ex_nonz_cap_to_def invs_valid_objs)
