proof/invariant-abstract/Tcb_AI.thy
@@ -11,7 +11,6 @@ begin
 arch_requalify_facts
   arch_derive_is_arch
   rec_del_invs''
-  as_user_valid_tcbs
 
 locale Tcb_AI_1 =
   fixes state_ext_t :: "'state_ext::state_ext itself"
